RocqOfRust/ruint/simulate/from.v
@@ -1,6 +1,8 @@
 Require Import RocqOfRust.RocqOfRust.
 Require Import RocqOfRust.links.M.
 Require Import RocqOfRust.simulate.M.
+Require Import core.convert.links.mod.
+Require Import core.convert.simulate.mod.
 Require Import core.links.result.
 Require Import ruint.links.from.
 Require Import ruint.links.lib.
@@ -12,7 +14,10 @@ Module UintTryFrom.
   }.
 
   Module Eq.
-    Class C (Self T : Set) `{Link Self} `{Link T} `{C Self T} `{!UintTryFrom.Run Self T} : Set := {
+    Class C {Self T : Set} `{Link Self} `{Link T}
+        `{run : !UintTryFrom.Run Self T}
+        `(!C Self T) :
+        Prop := {
       uint_try_from_eq (value : T) (stack : Stack.t) :
         {{
           SimulateM.eval_f
@@ -27,11 +32,61 @@ Module UintTryFrom.
   End Eq.
 End UintTryFrom.
 
+Module UintTryFrom_T_for_Uint_where_TryFrom.
+  Definition Self (BITS LIMBS : usize) : Set :=
+    Uint.t BITS LIMBS.
+
+  Definition uint_try_from {BITS LIMBS : usize} {T : Set}
+      `{!TryFrom.C (Self BITS LIMBS) T (ToUintError.t (Self BITS LIMBS))}
+      (value : T) :
+    Result.t (Self BITS LIMBS) (ToUintError.t (Self BITS LIMBS)) :=
+    TryFrom.try_from value.
+
+  Lemma uint_try_from_eq {BITS LIMBS : usize} {T : Set} `{Link T}
+      `{!TryFrom.Run (Self BITS LIMBS) T (ToUintError.t (Self BITS LIMBS))}
+      `{I : !TryFrom.C (Self BITS LIMBS) T (ToUintError.t (Self BITS LIMBS))}
+      `{H_TryFrom : !TryFrom.Eq.C I}
+      (value : T) (stack : Stack.t) :
+    {{
+      SimulateM.eval_f
+        (UintTryFrom_T_for_Uint_where_TryFrom.run_uint_try_from value)
+        stack 🌲
+      (
+        Output.Success (uint_try_from value),
+        stack
+      )
+    }}.
+  Proof.
+    eapply Run.Call. {
+      apply H_TryFrom.
+    }
+    apply Run.Pure.
+  Qed.
+
+  Instance I {BITS LIMBS : usize} {T : Set} `{Link T}
+      `(!TryFrom.C (Self BITS LIMBS) T (ToUintError.t (Self BITS LIMBS))) :
+    UintTryFrom.C (Self BITS LIMBS) T := {
+      uint_try_from := uint_try_from;
+    }.
+
+  Module Eq.
+    Instance I {BITS LIMBS : usize} {T : Set} `{Link T}
+      `{!TryFrom.Run (Self BITS LIMBS) T (ToUintError.t (Self BITS LIMBS))}
+      `{I_TryFrom : !TryFrom.C (Self BITS LIMBS) T (ToUintError.t (Self BITS LIMBS))}
+      `{!TryFrom.Eq.C I_TryFrom} :
+      UintTryFrom.Eq.C (I I_TryFrom) := {
+      uint_try_from_eq := uint_try_from_eq;
+    }.
+  End Eq.
+  Export (hints) Eq.
+End UintTryFrom_T_for_Uint_where_TryFrom.
+Export (hints) UintTryFrom_T_for_Uint_where_TryFrom.
+
 Module Impl_Uint.
   Definition Self (BITS LIMBS : usize) : Set :=
     Uint.t BITS LIMBS.
 
-  Definition from {BITS LIMBS : usize} {T : Set} `{UintTryFrom.C (Self BITS LIMBS) T}
+  Definition from {BITS LIMBS : usize} {T : Set} `{!UintTryFrom.C (Self BITS LIMBS) T}
       (value : T) :
       Self BITS LIMBS :=
     match UintTryFrom.uint_try_from value with
@@ -40,9 +95,9 @@ Module Impl_Uint.
     end.
 
   Lemma from_eq (BITS LIMBS : usize) (T : Set) `{Link T}
-      `{UintTryFrom.C (Self BITS LIMBS) T}
+      `{I_TryFrom : !UintTryFrom.C (Self BITS LIMBS) T}
       `{!UintTryFrom.Run (Self BITS LIMBS) T}
-      `{!UintTryFrom.Eq.C (Self BITS LIMBS) T}
+      `{H_TryFrom : !UintTryFrom.Eq.C I_TryFrom}
       (value : T) (stack : Stack.t)
       (H_success :
         match UintTryFrom.uint_try_from value with
@@ -62,14 +117,55 @@ Module Impl_Uint.
   Proof.
     with_strategy transparent [Impl_Uint.run_from] cbn.
     unfold from.
-    (* eapply Run.Call. {
-      apply UintTryFrom.Eq.uint_try_from_eq.
+    eapply Run.Call. {
+      apply H_TryFrom.
     }
-    destruct (_.(UintTryFrom.uint_try_from) value) as [n |]; cbn.
+    cbn.
+    destruct (I_TryFrom.(UintTryFrom.uint_try_from) value) as [n|e]; cbn.
     { apply Run.Pure. }
-    { easy. } *)
-  Admitted.
+    { easy. }
+  Qed.
 End Impl_Uint.
+
+Module TryFrom_bool_for_Uint.
+  Definition Self (BITS LIMBS : usize) : Set :=
+    Uint.t BITS LIMBS.
+
+  Definition Error (BITS LIMBS : usize) : Set :=
+    ToUintError.t (Self BITS LIMBS).
+
+  Definition try_from {BITS LIMBS : usize} (value : bool) :
+      Result.t (Self BITS LIMBS) (Error BITS LIMBS) :=
+    Result.Ok match value with
+    | true => {| Uint.value := 1 |}
+    | false => {| Uint.value := 0 |}
+  end.
+
+  Lemma try_from_eq {BITS LIMBS : usize} (value : bool) (stack : Stack.t) :
+    {{
+      SimulateM.eval_f
+        (TryFrom_bool_for_Uint.run_try_from BITS LIMBS value)
+        stack 🌲
+      (
+        Output.Success (try_from value),
+        stack
+      )
+    }}.
+  Proof.
+  Admitted.
+
+  Instance I (BITS LIMBS : usize) : TryFrom.C (Self BITS LIMBS) bool (Error BITS LIMBS) := {
+    try_from := try_from;
+  }.
+
+  Module Eq.
+    Instance I {BITS LIMBS : usize} : TryFrom.Eq.C (I BITS LIMBS) := {
+      try_from := try_from_eq;
+    }.
+  End Eq.
+  Export (hints) Eq.
+End TryFrom_bool_for_Uint.
+Export (hints) TryFrom_bool_for_Uint.
 
 Module TryFrom_Uint_for_u64.
   Definition Self : Set :=
