RocqOfRust/core/convert/simulate/mod.v
@@ -1,0 +1,37 @@
+Require Import RocqOfRust.RocqOfRust.
+Require Import RocqOfRust.links.M.
+Require Import RocqOfRust.simulate.M.
+Require Import core.convert.links.mod.
+Require Import core.links.result.
+
+(*
+pub trait TryFrom<T>: Sized {
+    type Error;
+    fn try_from(value: T) -> Result<Self, Self::Error>;
+}
+*)
+Module TryFrom.
+  Class C (Self T Error : Set) : Set := {
+    try_from (value : T) : Result.t Self Error;
+  }.
+
+  Module Eq.
+    Class C
+        {Self T Error : Set} `{Link Self} `{Link T} `{Link Error}
+        `{!TryFrom.Run Self T Error}
+        `(!C Self T Error) :
+        Prop := {
+      try_from (value : T) (stack : Stack.t) :
+        {{
+          SimulateM.eval_f
+            (TryFrom.run_try_from value)
+            stack 🌲
+          (
+            Output.Success (try_from value),
+            stack
+          )
+        }};
+    }.
+  End Eq.
+End TryFrom.
+Export (hints) TryFrom.
