RocqOfRust/core/simulate/cmp.v
@@ -1,0 +1,232 @@
+Require Import RocqOfRust.RocqOfRust.
+Require Import RocqOfRust.links.M.
+Require Import RocqOfRust.simulate.M.
+Require Import core.links.cmp.
+Require Export core.links.cmpOrdering.
+
+(*
+pub trait PartialEq<Rhs: ?Sized = Self> {
+    fn eq(&self, other: &Rhs) -> bool;
+    fn ne(&self, other: &Rhs) -> bool;
+}
+*)
+Module PartialEq.
+  Class C (Self Rhs : Set) : Set := {
+    eq (self : Self) (other : Rhs) : bool;
+    ne (self : Self) (other : Rhs) : bool;
+  }.
+
+  Module Eq.
+    Class C
+        (Self Rhs : Set) `{Link Self} `{Link Rhs}
+        `{!PartialEq.Run Self Rhs}
+        (I : C Self Rhs) :
+        Prop := {
+      eq (ref_self : '& Self) (ref_other : '& Rhs) (stack : Stack.t)
+          (self : Self) (other : Rhs) :
+        {{
+          SimulateM.eval_f
+            (PartialEq.run_eq ref_self ref_other)
+            stack 🌲
+          (
+            Output.Success (I.(eq) self other),
+            stack
+          )
+        }};
+      ne (ref_self : '& Self) (ref_other : '& Rhs) (stack : Stack.t)
+          (self : Self) (other : Rhs) :
+        {{
+          SimulateM.eval_f
+            (PartialEq.run_ne ref_self ref_other)
+            stack 🌲
+          (
+            Output.Success (I.(ne) self other),
+            stack
+          )
+        }};
+    }.
+  End Eq.
+  Export (hints) Eq.
+End PartialEq.
+Export (hints) PartialEq.
+
+(*
+pub trait Eq: PartialEq { }
+*)
+Module Eq.
+  Class C (Self : Set) : Set := {
+    PartialEq_for_Self :: PartialEq.C Self Self;
+  }.
+
+  Module Eq.
+    Class C
+        (Self : Set) `{Link Self}
+        `{!links.cmp.Eq.Run Self}
+        (I : C Self) :
+        Prop := {
+      PartialEq_for_Self :: PartialEq.Eq.C Self Self I.(PartialEq_for_Self);
+    }.
+  End Eq.
+  Export (hints) Eq.
+End Eq.
+Export (hints) Eq.
+
+(*
+pub trait Ord: Eq + PartialOrd<Self> {
+    fn cmp(&self, other: &Self) -> Ordering;
+    fn max(self, other: Self) -> Self;
+    fn min(self, other: Self) -> Self;
+    fn clamp(self, min: Self, max: Self) -> Self;
+}
+*)
+Module Ord.
+  Class C (Self : Set) : Set := {
+    cmp (self other : Self) : Ordering.t;
+    max (self other : Self) : Self;
+    min (self other : Self) : Self;
+    clamp (self min max : Self) : Self;
+  }.
+
+  Module Eq.
+    Class C
+        (Self : Set) `{Link Self}
+        `{!links.cmp.Ord.Run Self}
+        (I : C Self) :
+        Prop := {
+      cmp (ref_self ref_other : '& Self) (stack : Stack.t)
+          (self other : Self) :
+        {{
+          SimulateM.eval_f
+            (links.cmp.Ord.run_cmp ref_self ref_other)
+            stack 🌲
+          (
+            Output.Success (I.(cmp) self other),
+            stack
+          )
+        }};
+      max (self other : Self) (stack : Stack.t) :
+        {{
+          SimulateM.eval_f
+            (links.cmp.Ord.run_max self other)
+            stack 🌲
+          (
+            Output.Success (I.(max) self other),
+            stack
+          )
+        }};
+      min (self other : Self) (stack : Stack.t) :
+        {{
+          SimulateM.eval_f
+            (links.cmp.Ord.run_min self other)
+            stack 🌲
+          (
+            Output.Success (I.(min) self other),
+            stack
+          )
+        }};
+      clamp (self min max : Self) (stack : Stack.t) :
+        {{
+          SimulateM.eval_f
+            (links.cmp.Ord.run_clamp self min max)
+            stack 🌲
+          (
+            Output.Success (I.(clamp) self min max),
+            stack
+          )
+        }};
+    }.
+  End Eq.
+  Export (hints) Eq.
+End Ord.
+Export (hints) Ord.
+
+(*
+pub trait PartialOrd<Rhs: ?Sized = Self>: PartialEq<Rhs> {
+    fn partial_cmp(&self, other: &Rhs) -> Option<Ordering>;
+    fn lt(&self, other: &Rhs) -> bool;
+    fn le(&self, other: &Rhs) -> bool;
+    fn gt(&self, other: &Rhs) -> bool;
+    fn ge(&self, other: &Rhs) -> bool;
+}
+*)
+Module PartialOrd.
+  Class C (Self Rhs : Set) : Set := {
+    partial_cmp (self : Self) (other : Rhs) : option Ordering.t;
+    lt (self : Self) (other : Rhs) : bool;
+    le (self : Self) (other : Rhs) : bool;
+    gt (self : Self) (other : Rhs) : bool;
+    ge (self : Self) (other : Rhs) : bool;
+  }.
+
+  Module Eq.
+    Class C
+        (Self Rhs : Set) `{Link Self} `{Link Rhs}
+        `{!links.cmp.PartialOrd.Run Self Rhs}
+        (I : C Self Rhs) :
+        Prop := {
+      partial_cmp (ref_self : '& Self) (ref_other : '& Rhs) (stack : Stack.t)
+          (self : Self) (other : Rhs) :
+        {{
+          SimulateM.eval_f
+            (links.cmp.PartialOrd.run_partial_cmp ref_self ref_other)
+            stack 🌲
+          (
+            Output.Success (I.(partial_cmp) self other),
+            stack
+          )
+        }};
+      lt (ref_self : '& Self) (ref_other : '& Rhs) (stack : Stack.t) :
+        SimulateM.eval_f
+          (links.cmp.PartialOrd.run_lt ref_self ref_other)
+          stack =
+        let*s self := SimulateM.read stack ref_self.(Ref.core) in
+        match self with
+        | Output.Success self =>
+          let*s other := SimulateM.read stack ref_other.(Ref.core) in
+          match other with
+          | Output.Success other =>
+            SimulateM.Pure (Output.Success (lt self other), stack)
+          | Output.Exception exception =>
+            SimulateM.Pure (Output.Exception (R := bool) exception, stack)
+          end
+        | Output.Exception exception =>
+          SimulateM.Pure (Output.Exception (R := bool) exception, stack)
+        end;
+      le (ref_self : '& Self) (ref_other : '& Rhs) (stack : Stack.t)
+          (self : Self) (other : Rhs) :
+        {{
+          SimulateM.eval_f
+            (links.cmp.PartialOrd.run_le ref_self ref_other)
+            stack 🌲
+          (
+            Output.Success (le self other),
+            stack
+          )
+        }};
+      gt (ref_self : '& Self) (ref_other : '& Rhs) (stack : Stack.t)
+          (self : Self) (other : Rhs) :
+        {{
+          SimulateM.eval_f
+            (links.cmp.PartialOrd.run_gt ref_self ref_other)
+            stack 🌲
+          (
+            Output.Success (gt self other),
+            stack
+          )
+        }};
+      ge (ref_self : '& Self) (ref_other : '& Rhs) (stack : Stack.t)
+          (self : Self) (other : Rhs) :
+        {{
+          SimulateM.eval_f
+            (links.cmp.PartialOrd.run_ge ref_self ref_other)
+            stack 🌲
+          (
+            Output.Success (ge self other),
+            stack
+          )
+        }};
+    }.
+  End Eq.
+  Export (hints) Eq.
+End PartialOrd.
+Export (hints) PartialOrd.
